Add changes from meeting, start implementing completeness

theories/codes.v
@@ -1,4 +1,5 @@
 Require Import ssreflect ssrbool ssrfun.
+From HB Require Import structures.
 From mathcomp Require Import ssrnat eqtype div seq.
 
 (*
@@ -18,6 +19,7 @@ Proof.
   by move => word; rewrite /comparable prefix_refl.
 Qed.
 
+
 Lemma comparable_symm: forall word1 word2,
   comparable word1 word2 -> comparable word2 word1.
 Proof.
@@ -34,6 +36,8 @@ Qed.
 (* TODO(reiniscirpons): Maybe do sets? *)
 Definition binary_code := seq binary_word.
 
+(* TODO(reiniscirpons): Explicitly mention prefix codes are finite
+   in this development *)
 Fixpoint prefix_code (code: binary_code): bool :=
   match code with
   | nil => true
@@ -106,6 +110,21 @@ Inductive binary_tree :=
 | Empty: binary_tree
 | Node: binary_tree -> binary_tree -> binary_tree.
 
+Scheme Equality for binary_tree.
+
+Lemma binary_tree_eqP: forall (tree1 tree2: binary_tree),
+  reflect (tree1 = tree2) (binary_tree_beq tree1 tree2).
+Proof.
+  move => tree1 tree2.
+  apply (iffP idP).
+  - elim: tree1 tree2 => [ | l Hl r Hr]; case => //.
+    by move => l2 r2 /= /andP [] /Hl <- /Hr <-.
+  - move => <-; elim: tree1 => [//|l Hl r Hr /=].
+    by rewrite Hl Hr. 
+Qed.
+
+HB.instance Definition _ :=
+  hasDecEq.Build binary_tree binary_tree_eqP.
 
 (* Luna attempt at making the free jonsson tarski algeba. the node operator is usually called 
 lambda in the literature and the child operators are usually called alpha_0 alpha_1. dont know if 
@@ -142,7 +161,8 @@ Fixpoint jt_reduce_exp (t : jt_expression) : jt_expression :=
       end
   end.
 
-Definition is_reduced_jt (t : jt_expression) : Prop := jt_reduce_exp t = t.
+Definition is_reduced_jt (t : jt_expression) : Prop :=
+  jt_reduce_exp t = t.
 
 Lemma jt_reduction_is_idempotent (t : jt_expression) : is_reduced_jt (jt_reduce_exp t).
 Proof.
@@ -153,7 +173,7 @@ reflexivity.
 Admitted.
 
 Record jt := {
-  normal_form : jt_expression;
+  normal_form :> jt_expression;
   is_normal_form : is_reduced_jt normal_form;
 }.
 
@@ -181,8 +201,6 @@ Definition JTRight (n : jt) : jt :=
 
 Definition JTeq (x : jt) (y : jt) : bool := jt_expression_beq (normal_form x) (normal_form y).
 
-
-
 Definition Leaf := Node Empty Empty.
 Definition Caret := Node Leaf Leaf.
 
@@ -201,6 +219,35 @@ Fixpoint add_word (tree: binary_tree) (word: binary_word): binary_tree :=
     end
   end.
 
+Fixpoint any_leaf (tree:binary_tree): option binary_word :=
+  match tree with
+  | Empty => None
+  | Node l r =>
+    match any_leaf l with
+    | None => match any_leaf r with
+      | None => None
+      | Some w => Some (true::w)
+      end
+    | Some w => Some (false::w)
+    end
+  end.
+
+Fixpoint follow_word (tree: binary_tree) (word: binary_word):
+  option binary_word :=
+    match tree, word with
+    | Empty, _ => None
+    | _, nil => any_leaf tree
+    | Node l r, false::word' =>
+      match follow_word l word' with
+      | None => None
+      | Some lw' => Some (false::lw')
+      end
+    | Node l r, true::word' =>
+      match follow_word r word' with
+      | None => None
+      | Some rw' => Some (false::rw')
+      end
+    end.
 
 Fixpoint tree_of_code (code: binary_code): binary_tree :=
   match code with
@@ -246,6 +293,29 @@ Proof.
   elim => [//|l Hl r Hr] /=.
 Admitted.
 
+Fixpoint complete_tree (tree: binary_tree): bool :=
+  match tree with
+  | Empty => false
+  | Node l r =>
+    ((l == Empty) && (r == Empty)) ||
+    (complete_tree l && complete_tree r)
+  end.
+
+Definition is_complete (P: binary_code): Prop :=
+  (prefix_code P) /\
+  (forall (u: binary_word), exists (v: binary_word),
+   v \in P /\ comparable u v).
+
+Definition complete (P: binary_code): bool :=
+  (prefix_code P) && (complete_tree (tree_of_code P)).
+
+Lemma completeP: forall P,
+  reflect (is_complete P) (complete P).
+Proof.
+  move => P; apply (iffP andP).
+  - case => HP Htree; split => [//|u].
+    pose v := (follow_word (tree_of_code P) u).
+Admitted.
 
 
 
